parameterize Distance over an equiv

theories/diffpriv/diffpriv_rules.v
@@ -9,39 +9,42 @@ Section diffpriv.
 
   #[local] Open Scope R.
 
-  Class Distance A := { carrier :: Inject A val
+  Class Distance A := { distance_car :: Inject A val
+                      ; distance_equiv :: Equiv A
                       ; distance : A -> A -> R
                       ; distance_pos a1 a2 : 0 <= distance a1 a2
-                      ; distance_0 a : distance a a = 0
-                      ; distance_sep a1 a2 : distance a1 a2 <= 0 -> a1 = a2
+                      ; distance_0 a1 a2 : a1 ≡ a2 → distance a1 a2 = 0
+                      ; distance_sep a1 a2 : distance a1 a2 <= 0 -> a1 ≡ a2
                       (* leaving out symmetry and triangle inequality until they're needed. *)
                       (* ; distance_sym a1 a2 : distance a1 a2 = distance a2 a1 *)
                       (* ; distance_triangle a1 a2 a3 : distance a1 a3 <= distance a1 a2 + distance a2 a3 *)
     }.
-  Arguments carrier {_} _.
-  Coercion carrier : Distance >-> Inject.
+  Arguments distance_car {_} _.
+  Coercion distance_car : Distance >-> Inject.
   Arguments distance {_} _ _ _.
   Coercion distance : Distance >-> Funclass.
 
-  Program Definition dZ : Distance Z := {| distance z z' := Rabs (IZR (z - z')) |}.
+  Program Definition dZ : Distance Z := {| distance z z' := Rabs (IZR (z - z')); distance_equiv := (=) |}.
   Next Obligation. intros => /= ; eauto using Rabs_pos. Qed.
-  Next Obligation. intros => /= ; replace (a - a)%Z with 0%Z by lia. exact Rabs_R0. Qed.
+  Next Obligation. intros ?? -> => /=; replace (a2 - a2)%Z with 0%Z by lia. exact Rabs_R0. Qed.
   Next Obligation.
     intros ?? => /= ; rewrite -abs_IZR. pose proof (IZR_le _ _ $ Zabs_pos (a1-a2)).
     intros h. assert (IZR (Z.abs (a1 - a2)) = 0) as h' by lra. revert h'.
-    apply Zabs_ind ; intros ? h' ; apply eq_IZR in h' ; lia.
+    rewrite /equiv. apply Zabs_ind ; intros ? h' ; apply eq_IZR in h' ; lia.
   Qed.
 
   Program Definition dtensor `(dA : Distance A) `(dB : Distance B) : Distance (A * B) :=
-    {| distance x y := let (x1, x2) := x in let (y1, y2) := y in dA x1 y1 + dB x2 y2 |}.
+    {| distance x y := let (x1, x2) := x in let (y1, y2) := y in dA x1 y1 + dB x2 y2;
+       distance_equiv x y := let (x1, x2) := x in let (y1, y2) := y in x1 ≡ y1 ∧ x2 ≡ y2;
+    |}.
   Next Obligation. intros ???? [] []. apply Rplus_le_le_0_compat ; apply distance_pos. Qed.
-  Next Obligation. intros ???? []. rewrite !distance_0. lra. Qed.
+  Next Obligation. intros ???? [] [] []. rewrite !distance_0 //. lra. Qed.
   Next Obligation.
     intros ???? [a b] [a' b'] ?.
     pose proof (distance_pos a a'). pose proof (distance_pos b b').
     assert (dA a a' <= 0) by lra. assert (dB b b' <= 0) by lra.
     pose proof (distance_sep a a'). pose proof (distance_sep b b').
-    f_equal ; intuition auto.
+    rewrite /equiv. intuition auto.
   Qed.
 
   Definition wp_sensitive (f : expr) (c : R) `(d_in : Distance A) `(d_out : Distance B) : iProp Σ
@@ -65,25 +68,28 @@ Section diffpriv.
                       ∧ ⌜d_out b b' <= c * d_in x x'⌝
       }}}.
 
-  Definition wp_diffpriv (f : expr) ε δ `(dA : Distance A) : iProp Σ := ∀ K c (x x' : A), ⌜dA x x' <= c⌝ →
+  Definition wp_diffpriv (f : expr) ε δ `(dA : Distance A) `(dB : Distance B) : iProp Σ :=
+    ∀ K c (x x' : A), ⌜dA x x' <= c⌝ →
     ⤇ fill K (f (Val (inject x'))) ∗ ↯m (c * ε) ∗ ↯(c * δ) -∗
-      WP f (Val (inject x)) {{ v, ⤇ fill K (Val v) }}.
+      WP f (Val (inject x)) {{ v, ∃ (y y' : B), ⌜v = inject y⌝ ∗ ⌜y ≡ y'⌝ ∗ ⤇ fill K (inject y') }}.
 
-  Definition wp_diffpriv_pw (f : expr) ε δ `(dA : Distance A) : iProp Σ := ∀ K c (x x' : A), ⌜dA x x' <= c⌝ →
+  Definition wp_diffpriv_pw (f : expr) ε δ `(dA : Distance A) `(dB : Distance B) : iProp Σ :=
+    ∀ K c (x x' : A), ⌜dA x x' <= c⌝ →
     ⤇ fill K (f (Val (inject x'))) ∗ ↯m (c * ε) ∗ ↯(c * δ) -∗
-    ∀ r,
-      WP f (Val (inject x)) {{ v, ∃ (v' : val), ⤇ fill K (Val v') ∗ ⌜v = r → v' = r⌝ }}.
+    ∀ (r : B),
+      WP f (Val (inject x)) {{ v, ∃ (y y' : B), ⌜v = inject y⌝ ∗ ⌜y ≡ y'⌝ ∗ ⤇ fill K (inject y') ∗ ⌜y = r → y' = r⌝ }}.
 
-  Definition hoare_diffpriv (f : expr) ε δ `(dA : Distance A) : iProp Σ := ∀ K c (x x' : A), ⌜dA x x' <= c⌝ →
+  Definition hoare_diffpriv (f : expr) ε δ `(dA : Distance A) `(dB : Distance B) : iProp Σ :=
+    ∀ K c (x x' : A), ⌜dA x x' <= c⌝ -∗
       {{{ ⤇ fill K (f (Val (inject x'))) ∗ ↯m (c * ε) ∗ ↯ (c * δ) }}}
         f (Val (inject x))
-      {{{ (v : val), RET v; ⤇ fill K (Val v) }}}.
+      {{{ (y y' : B), RET (inject y); ⌜y ≡ y'⌝ ∗ ⤇ fill K (inject y') }}}.
 
-  Lemma wp_diffpriv_mono (f : val) ε δ ε' δ' `(dA : Distance A)
+  Lemma wp_diffpriv_mono (f : val) ε δ ε' δ' `(dA : Distance A) `(dB : Distance B)
     (ε_pos : 0 <= ε) (hε' : ε <= ε')
     (δ_pos : 0 <= δ) (hδ' : δ <= δ') :
-    wp_diffpriv f ε δ dA -∗
-    wp_diffpriv f ε' δ' dA.
+    wp_diffpriv f ε δ dA dB -∗
+    wp_diffpriv f ε' δ' dA dB.
   Proof.
     iIntros "fεδ" (?? a a' ?) "[rhs [ε δ]]".
     pose proof (distance_pos a a').
@@ -109,14 +115,14 @@ Section diffpriv.
 
   Fact hoare_laplace_diffpriv (num den : Z) :
     ⌜0 < IZR num / IZR den⌝ -∗
-    hoare_diffpriv (λ: "loc", Laplace #num #den "loc")%E ((IZR num / IZR den)) 0 dZ.
+    hoare_diffpriv (λ: "loc", Laplace #num #den "loc")%E ((IZR num / IZR den)) 0 dZ dZ.
   Proof.
     iIntros. rewrite /hoare_diffpriv/dZ /=. iIntros (K c x x' adj).
     iIntros (φ) "!> [f' [ε δ]] hφ".
     tp_pures. wp_pures.
     tp_bind (Laplace _ _ _).
     iApply (hoare_couple_laplace _ _ 0%Z with "[$f' ε]") => //.
-    2: setoid_rewrite Z.add_0_r ; iNext ; iIntros ; iApply "hφ" ; iFrame.
+    2: setoid_rewrite Z.add_0_r ; iNext ; iIntros ; iApply "hφ" ; iFrame ; done.
     iFrame. iApply ecm_weaken. 2: iFrame.
     split. all: rewrite abs_IZR ; real_solver_partial. 1: apply Rabs_pos.
     3: rewrite Z.add_0_l. all: lra.
@@ -143,7 +149,7 @@ Section diffpriv.
   Fact diffpriv_sensitive_comp (f g : val) ε δ c
     `(dA : Distance A) `(dB : Distance B) {C : Type} `(dC : Distance C)
     (c_pos : 0 <= c) :
-    hoare_sensitive f c dA dB -∗ hoare_diffpriv g ε δ dB -∗ hoare_diffpriv (λ:"x", g (f "x")) (c*ε) (c*δ) dA.
+    hoare_sensitive f c dA dB -∗ hoare_diffpriv g ε δ dB dC -∗ hoare_diffpriv (λ:"x", g (f "x")) (c*ε) (c*δ) dA dC.
   Proof.
     rewrite /hoare_sensitive/hoare_diffpriv. iIntros "#f_sens #g_dipr". iIntros (K c'). iIntros. iIntros (Φ) "!> [f' [ε δ]] hΦ".
     wp_pures. wp_bind (f _). tp_pures. tp_bind (f _).
@@ -151,14 +157,15 @@ Section diffpriv.
     iIntros "!>" (_v) "(%v & %v' & -> & gv' & %sens)".
     iApply ("g_dipr" $! K (c * c') _ _ _ with "[$gv' ε δ]").
     { rewrite (Rmult_comm c c') 2!Rmult_assoc. iFrame. }
-    Unshelve. 1-2: done.
+    Unshelve.
+    1-2 : done.
     etrans => //. apply Rmult_le_compat_l => //.
   Qed.
 
   Fact diffpriv_pw_sensitive_comp (f g : val) ε δ c
     `(dA : Distance A) `(dB : Distance B) {C : Type} `(dC : Distance C)
     (c_pos : 0 <= c) :
-    wp_sensitive f c dA dB -∗ wp_diffpriv_pw g ε δ dB -∗ wp_diffpriv_pw (λ:"x", g (f "x")) (c*ε) (c*δ) dA.
+    wp_sensitive f c dA dB -∗ wp_diffpriv_pw g ε δ dB dC -∗ wp_diffpriv_pw (λ:"x", g (f "x")) (c*ε) (c*δ) dA dC.
   Proof.
     rewrite /wp_sensitive/wp_diffpriv_pw. iIntros "f_sens g_dipr". iIntros (K c'). iIntros (??) "% [f' [ε δ]] %".
     wp_pures. wp_bind (f _). tp_pures. tp_bind (f _).
@@ -170,60 +177,56 @@ Section diffpriv.
     etrans. 1: eauto. real_solver.
   Qed.
 
-  Definition hoare_functional_on (A : Type) {_ : Inject A val} (f : expr) : iProp Σ := ∀ K (x : A) ,
-    {{{ ⤇ fill K (f $ Val $ inject x) }}}
+  Definition hoare_functional_on `(dA : Distance A) `(dB: Distance B) (f : expr) : iProp Σ := ∀ K (x x' : A) ,
+    ⌜x ≡ x'⌝ -∗
+    {{{ ⤇ fill K (f $ Val $ inject x') }}}
       f $ Val $ inject x
-      {{{ (v : val), RET v; ⤇ fill K (Val v) }}}.
+    {{{ (y y' : B), RET (inject y); ⌜y ≡ y'⌝ ∗ ⤇ fill K (inject y') }}}.
 
   Definition hoare_has_codomain (B : Type) {_ : Inject B val} (f : expr) : iProp Σ :=
     ∀ x P Q, {{{ P }}} f x {{{ v , RET v ; Q v }}} -∗ {{{ P }}} f x {{{ v , RET v ; ∃ b, ⌜ v = inject b ⌝ ∧ Q v }}}.
 
-  Fact well_typed_diffpriv_comp (f g : val) ε δ c `(dA : Distance A) `(dB : Distance B) (c_pos : 0 <= c) :
-    hoare_diffpriv f ε δ dA -∗ hoare_has_codomain B f -∗ hoare_functional_on B g -∗ hoare_diffpriv (λ:"x", g (f "x")) ε δ dA.
+  Fact well_typed_diffpriv_comp (f g : val) ε δ c `(dA : Distance A) `(dB : Distance B) `(dC : Distance D) (c_pos : 0 <= c) :
+    hoare_diffpriv f ε δ dA dB -∗ hoare_has_codomain B f -∗ hoare_functional_on dB dC g -∗ hoare_diffpriv (λ:"x", g (f "x")) ε δ dA dC.
   Proof.
     rewrite /hoare_sensitive/hoare_diffpriv. iIntros "#f_dipr f_cod #g_dom". iIntros (K c' ?? adj ?).
-    iSpecialize (("f_dipr" $! _ c' _ _ _)).
-    iPoseProof ("f_cod" with "[$f_dipr]") as "#Hg".
     iIntros "!> [g [ε δ]] hΦ".
     wp_pures. wp_bind (f _). tp_pures. tp_bind (f _).
-    iApply ("Hg" with "[$g ε δ]") => //; [iFrame|].
-    iNext. iIntros (?) "(%gix & -> & f')".
-    iApply ("g_dom" with "[$f']").
-    iIntros "!>" (?) "gv'".
-    iApply "hΦ". done.
-    Unshelve. auto.
+    iApply ("f_dipr" with "[//] [f_dipr $g $ε $δ]").
+    iIntros "!>" (y y') "[% g]".
+    rewrite /hoare_functional_on.
+    by iApply ("g_dom" with "[] g").
   Qed.
 
-  Fact diffpriv_functional (f : val) ε δ `(dA : Distance A) :
-    hoare_diffpriv f ε δ dA -∗ hoare_functional_on A f.
+  Fact diffpriv_functional (f : val) ε δ `(dA : Distance A) `(dB : Distance B) :
+    hoare_diffpriv f ε δ dA dB -∗ hoare_functional_on dA dB f.
   Proof.
-    iIntros "#f_dipr" (K z Φ) "!> fz hΦ".
+    iIntros "#f_dipr" (K z z' Φ) "!> % fz hΦ".
     iMod ecm_zero as "ε0".
     iMod ec_zero as "δ0".
     rewrite /hoare_diffpriv.
     unshelve iApply ("f_dipr" $! K 0 _ _ _ with "[$fz ε0 δ0]") => //.
-    - right ; apply distance_0.
+    - right ; by apply distance_0.
     - rewrite 2!Rmult_0_l. iFrame.
   Qed.
 
   Fact sensitive_functional (f : val) c `(dA : Distance A) `(dB : Distance B) (c_pos : 0 <= c) :
-    hoare_sensitive f c dA dB -∗ hoare_functional_on A f.
+    hoare_sensitive f c dA dB -∗ hoare_functional_on dA dB f.
   Proof.
-    iIntros "#f_sens" (K z Φ) "!> f' hΦ".
+    iIntros "#f_sens" (K z z' Φ) "!> % f' hΦ".
     rewrite /hoare_sensitive.
     iApply ("f_sens" $! c_pos K with "[$f']").
     iNext. iIntros (v) "(%b & %b' & -> & b' & %sens)".
-    iApply "hΦ".
-    assert (b = b') as -> => //.
+    iApply "hΦ". iFrame. iPureIntro.
     move: sens.
-    rewrite distance_0. rewrite Rmult_0_r. apply distance_sep.
+    rewrite (distance_0 z) //. rewrite Rmult_0_r. apply distance_sep.
   Qed.
 
   Corollary diffpriv_diffpriv_comp (f g : val) εf δf εg δg
     `(dA : Distance A) `(dB : Distance B) {C : Type} `(dC : Distance C)
     (εg_pos : 0 <= εg) (δg_pos : 0 <= δg) (εf_pos : 0 <= εf) (δf_pos : 0 <= δf) :
-    hoare_has_codomain B f -∗ hoare_diffpriv f εf δf dA -∗
-    hoare_diffpriv g εg δg dB -∗ hoare_diffpriv (λ:"x", g (f "x")) εf δf dA.
+    hoare_has_codomain B f -∗ hoare_diffpriv f εf δf dA dB -∗
+    hoare_diffpriv g εg δg dB dC -∗ hoare_diffpriv (λ:"x", g (f "x")) εf δf dA dC.
   Proof.
     iIntros "f_cod #f_dipr #g_dipr". iIntros (???? h).
     iPoseProof (diffpriv_functional _ _ _ with "g_dipr") as "g_fun".
@@ -233,13 +236,12 @@ Section diffpriv.
 
   Corollary sensitive_diffpriv_comp (g f : val) ε δ c (c_pos : 0 <= c)
     `(dA : Distance A) `(dB : Distance B) {C : Type} `(dC : Distance C) :
-    hoare_diffpriv f ε δ dA -∗ hoare_has_codomain B f -∗
-    hoare_sensitive g c dB dC -∗ hoare_diffpriv (λ:"x", g (f "x")) ε δ dA.
+    hoare_diffpriv f ε δ dA dB -∗ hoare_has_codomain B f -∗
+    hoare_sensitive g c dB dC -∗ hoare_diffpriv (λ:"x", g (f "x")) ε δ dA dC.
   Proof.
     iIntros "#f_dipr f_cod #g_sens".
-    iPoseProof (sensitive_functional _ _ _ _ _ with "g_sens") as "g_fun" => //.
-    iApply (well_typed_diffpriv_comp _ _ _ _ _ _ _ c_pos with "f_dipr f_cod g_fun").
-    Unshelve. auto.
+    iPoseProof (sensitive_functional with "g_sens") as "g_fun" => //.
+    by iApply (well_typed_diffpriv_comp with "f_dipr f_cod g_fun").
   Qed.
 
   (* The typing here is a bit weird with `f : A → B` and `g : B → A → C` ; it
@@ -247,11 +249,11 @@ Section diffpriv.
   has to refer to g's last argument, and reasoning about `λ a, g a b` is
   annoying. *)
   Theorem diffpriv_diffpriv_seq_comp (f g : val) εf δf εg δg
-    `(dA : Distance A) `(dB : Distance B)
+    `(dA : Distance A) `(dB : Distance B) {C : Type} `(dC : Distance C)
     (εg_pos : 0 <= εg) (δg_pos : 0 <= δg) (εf_pos : 0 <= εf) (δf_pos : 0 <= δf):
-    hoare_diffpriv f εf δf dA -∗
-    (∀ b, hoare_diffpriv (g b) εg δg dA) -∗
-    hoare_diffpriv (λ:"a", g (f "a") "a") (εf+εg) (δf+δg) dA.
+    hoare_diffpriv f εf δf dA dB -∗
+    (∀ b, hoare_diffpriv (g b) εg δg dA dC) -∗
+    hoare_diffpriv (λ:"a", g (f "a") "a") (εf+εg) (δf+δg) dA dC.
   Proof.
     iIntros "#f_dipr #g_dipr" (?? a a' adj Φ) "!> [gfa' [ε δ]] HΦ".
     rewrite 2!Rmult_plus_distr_l.
@@ -259,18 +261,24 @@ Section diffpriv.
     iDestruct (ecm_split with "ε") as "[εf εg]" => //. 1,2: real_solver.
     iDestruct (ec_split with "δ") as "[δf δg]" => //. 1,2: real_solver.
     tp_pures ; wp_pures. tp_bind (f _). wp_bind (f _).
-    iApply ("f_dipr" $! _ _ _ _ _ with "[$gfa' $εf $δf]") => // ; iIntros "!>" (b) "gb" => /=.
-    iSpecialize ("g_dipr" $! b K c a a' adj with "[$gb $εg $δg]").
-    iApply "g_dipr". done.
-    Unshelve. auto.
-  Qed.
+    iApply ("f_dipr" $! _ _ _ _ _ with "[$gfa' $εf $δf]") => //.
+    iIntros "!>" (b b') "[% gb]" => /=.
+    iEval (rewrite /hoare_diffpriv) in "g_dipr".
+    iSpecialize ("g_dipr" $! _ K c a a' adj with "[$gb $εg $δg]").
+
+    (* TODO: I think [hoare_diffpriv] might need to be generalized to two programs so the input can
+       be varied (i.e. [b] on one side and [b'] on the other? *)
+    (* iApply "g_dipr". done. *)
+    (* Unshelve. auto. *)
+  Admitted.
+  (* Qed. *)
 
   Theorem wp_diffpriv_diffpriv_par_comp (f g : val) ε δ
-    `(dA : Distance A) `(dB : Distance B)
+    `(dA : Distance A) `(dB : Distance B) {C : Type} `(dC : Distance C) `(dD : Distance D)
     (ε_pos : 0 <= ε) (δ_pos : 0 <= δ) :
-    wp_diffpriv f ε δ dA -∗
-    wp_diffpriv g ε δ dB -∗
-    wp_diffpriv (λ:"xy", (f (Fst "xy"), g (Snd "xy"))) ε δ (dtensor dA dB).
+    wp_diffpriv f ε δ dA dC -∗
+    wp_diffpriv g ε δ dB dD -∗
+    wp_diffpriv (λ:"xy", (f (Fst "xy"), g (Snd "xy"))) ε δ (dtensor dA dB) (dtensor dC dD).
   Proof.
     iIntros "f_dipr g_dipr" (?? [a b] [a' b'] adj) "[fa_gb' [ε δ]]".
     rewrite /dtensor in adj. simpl in adj.
@@ -282,20 +290,22 @@ Section diffpriv.
     tp_pures ; wp_pures. tp_bind (g _). wp_bind (g _).
     iApply (wp_strong_mono'' with "[g_dipr fa_gb' εg δg] [-]").
     1: iApply "g_dipr". 2: iFrame. 1: iPureIntro ; lra.
-    iIntros (gb) "rhs /=". tp_pures. wp_pures.
+    iIntros (gb) "(%y & %y' & -> & % & rhs) /=". tp_pures. wp_pures.
     tp_bind (f _) ; wp_bind (f _).
     iApply (wp_strong_mono'' with "[f_dipr rhs εf δf] [-]").
     1: iApply "f_dipr". 2: iFrame. 1: iPureIntro ; lra.
-    iIntros (fa) "rhs /=". tp_pures. wp_pures.
+    iIntros (fa) "(%z & %z' & -> & % & rhs) /=".
+    tp_pures. wp_pures.
+    iModIntro. iExists (_, _), (_,_). iFrame.
     done.
   Qed.
 
   Theorem diffpriv_diffpriv_par_comp (f g : val) ε δ
-    `(dA : Distance A) `(dB : Distance B)
+    `(dA : Distance A) `(dB : Distance B) {C : Type} `(dC : Distance C) `(dD : Distance D)
     (ε_pos : 0 <= ε) (δ_pos : 0 <= δ) :
-    hoare_diffpriv f ε δ dA -∗
-    hoare_diffpriv g ε δ dB -∗
-    hoare_diffpriv (λ:"xy", (f (Fst "xy"), g (Snd "xy"))) ε δ (dtensor dA dB).
+    hoare_diffpriv f ε δ dA dC -∗
+    hoare_diffpriv g ε δ dB dD -∗
+    hoare_diffpriv (λ:"xy", (f (Fst "xy"), g (Snd "xy"))) ε δ (dtensor dA dB) (dtensor dC dD).
   Proof.
     iIntros "#f_dipr #g_dipr" (?? [a b] [a' b'] adj Φ) "!> [fa_gb' [ε δ]] HΦ".
     rewrite /dtensor in adj. simpl in adj.
@@ -305,12 +315,13 @@ Section diffpriv.
     iDestruct (ec_weaken _ ((dA a a' + dB b b') * δ) with "δ") as "δ". 1: real_solver.
     rewrite Rmult_plus_distr_r. iDestruct (ec_split with "δ") as "[δf δg]" => //. 1,2: real_solver.
     tp_pures ; wp_pures. tp_bind (g _). wp_bind (g _).
-    iApply ("g_dipr" $! _ _ _ _ _ with "[$fa_gb' $εg $δg]") => // ; iIntros "!>" (gb) "fa_gb" => /=.
+    iApply ("g_dipr" $! _ _ _ _ _ with "[$fa_gb' $εg $δg]") => //.
+    iIntros "!>" (y y') "[% fa_gb]" => /=.
     tp_pures. wp_pures. tp_bind (f _). wp_bind (f _).
-    iApply ("f_dipr" $! _ _ _ _ _ with "[$fa_gb $εf $δf]") => // ; iIntros "!>" (fa) "fa_gb" => /=.
-    tp_pures. wp_pures. iApply "HΦ". done.
+    iApply ("f_dipr" $! _ _ _ _ _ with "[$fa_gb $εf $δf]") => //.
+    iIntros "!>" (z z') "[% fa_gb]" => /=.
+    tp_pures. wp_pures. iApply ("HΦ" $! (_, _) (_, _)). by iFrame.
     Unshelve. all: lra.
   Qed.
-
 
 End diffpriv.
